Split Effect.v into multiple files

Coq/src/DataM.v
@@ -1,5 +1,186 @@
-Require Import Thesis.Container.
-Require Import Thesis.Free.
+Require Import Thesis.Prog.
 Require Import Thesis.Base.
+Require Import Thesis.Effect.
+Require Import Thesis.Classes.
 
 Set Implicit Arguments.
+
+Section Prim.
+  Definition Coin : Prog nat := Choice None (pure 0) (pure 1).
+  Definition Coin__Bool : Prog bool := Choice None (pure true) (pure false).
+  
+  Definition addM (fn1 fn2 : Prog nat) : Prog nat :=
+    fn1 >>= fun n1 => fn2 >>= fun n2 => pure (n1 + n2).
+  
+  Definition orM (fn1 fn2 : Prog bool) : Prog bool :=
+    fn1 >>= fun b => match b with
+                  | true => pure true
+                  | false => fn2
+                  end.
+  
+  Definition duplicate A (fx : Prog A) : Prog (A * A) :=
+    fx >>= fun x => fx >>= fun y => pure (x,y).
+
+  Global Instance shareable__Nat : Shareable nat :=
+    {
+      shareArgs := pure
+    }.
+  
+  Global Instance shareable__Bool : Shareable bool :=
+    {
+      shareArgs := pure
+    }.
+  
+  Global Instance normalform__Nat : Normalform nat nat :=
+    {
+      nf := fun x => x
+    }.
+  
+  Global Instance normalform__Bool : Normalform bool bool :=
+    {
+      nf := fun x => x
+    }.
+End Prim.
+
+Section Pair.
+  Inductive Pair A B :=
+  | Pair' : Prog A -> Prog B -> Pair A B.
+  
+  Definition pairM A B (fst : Prog A) (snd : Prog B) : Prog (Pair A B) :=
+    pure (Pair' fst snd).
+
+  Definition firstM A B (fp : Prog (Pair A B)) : Prog A :=
+    fp >>= fun '(Pair' fst _) => fst.
+
+  Definition secondM A B (fp : Prog (Pair A B)) : Prog B :=
+    fp >>= fun '(Pair' _ snd) => snd.
+
+  Definition dup' (fp : Prog (Pair bool bool)) : Prog (Pair bool bool) :=
+    pairM (firstM fp) (firstM fp).
+
+  Definition dup A (fx : Prog A) : Prog (Pair A A) :=
+    pairM fx fx.
+
+  Definition dupShare A `{Shareable A} (fx : Prog A) : Prog (Pair A A) :=
+    Share fx >>= fun x => pairM x x.
+
+  Definition shrrgs__Pair A B `(Shareable A) `(Shareable B) (p : Pair A B) : Prog (Pair A B) :=
+    match p with
+    | Pair' a b => Share a >>= fun sa => Share b >>= fun sb => pairM sa sb
+    end.
+
+  Global Instance shareable__Pair A B `(sa : Shareable A) `(sb : Shareable B) : Shareable (Pair A B) :=
+    {
+      shareArgs := @shrrgs__Pair A B sa sb
+    }.
+
+  Definition nf__Pair A B C D `{Normalform A C} `{Normalform B D} (stp : Prog (Pair A B)) : Prog (Pair C D) :=
+    stp >>= fun '(Pair' sp1 sp2) =>
+              nf sp1 >>= fun b1 =>
+                           nf sp2 >>= fun b2 =>
+                                        pairM (pure b1) (pure b2).
+
+  Global Instance normalform__Pair A B C D `{Normalform A C} `{Normalform B D} : Normalform (Pair A B) (Pair C D) :=
+    {
+      nf := fun x => nf__Pair x
+    }.
+
+End Pair.
+
+Section List.
+  Inductive List A :=
+  | Nil' : List A
+  | Cons' : Prog A -> Prog (List A) -> List A.
+
+  Definition consM A (fx : Prog A) (fxs : Prog (List A)) : Prog (List A) :=
+    pure (Cons' fx fxs).
+
+  Definition nilM {A} : Prog (List A) := pure (@Nil' A).
+
+  Definition headM A (fxs : Prog (List A)) : Prog A :=
+    fxs >>= fun xs => match xs with
+                   | Nil' _    => @Fail A
+                   | Cons' x _ => x
+                   end.
+
+  Definition dupl A (fx : Prog A) : Prog (List A) :=
+    consM fx (consM fx (@nilM A)).
+
+  Definition duplShare A `{Shareable A} (fx : Prog A) : Prog (List A) :=
+    Share fx >>= fun x => consM x (consM x (@nilM A)).
+
+  Fixpoint appM' A (xs : List A) (fxs : Prog (List A)) : Prog (List A) :=
+    match xs with
+    | Nil' _       => fxs
+    | Cons' fz fzs => consM fz (fzs >>= fun zs => appM' zs fxs)
+    end.
+
+  Definition appM A (fxs fys : Prog (List A)) : Prog (List A) :=
+    fxs >>= fun xs => appM' xs fys.
+
+
+  Definition shrrgs__List A `(Shareable A) `(Shareable (List A)) (xs : List A) : Prog (List A) :=
+    match xs with
+    | Nil' _     => @nilM A
+    | Cons' y ys => Share y >>= fun sy => Share ys >>= fun sys => consM sy sys
+    end.
+
+  Global Instance shareable__List A `(sa : Shareable A) : Shareable (List A) :=
+    {
+      shareArgs := fun xs =>
+                     let fix aux xs :=
+                         let shr fp := Get >>= fun i =>
+                                       Put (i * 2) >>= fun _ =>
+                                       pure (Share' i (
+                                         Put (i * 2 + 1) >>= fun _ =>
+                                         fp >>= fun x => aux x))
+                         in
+                         match xs with
+                         | Nil' _     => @nilM A
+                         | Cons' y ys => Share y >>= fun sy => shr ys >>= fun sys => consM sy sys
+                         end
+                     in aux xs
+    }.
+
+  Fixpoint nf'__List A B `{Normalform A B} (xs : List A) : Prog (List B) :=
+    match xs with
+    | Nil' _ => nilM
+    | Cons' sx sxs => nf sx >>= fun x =>
+                                 sxs >>= fun xs => nf'__List xs >>= fun xs' =>
+                                                                 consM (pure x) (pure xs')
+    end.
+
+  Definition nf__List A B `{Normalform A B}  (stxs : Prog (List A)) : Prog (List B) :=
+    stxs >>= fun xs => nf'__List xs.
+
+  Global Instance normalform__List A B `{Normalform A B} : Normalform (List A) (List B) :=
+    {
+      nf := fun x => nf__List x
+    }.
+
+  Fixpoint lengthM A (xs : List A) : Prog nat :=
+    match xs with
+    | Nil' _ => pure 0
+    | Cons' _ fxs =>
+      let m := match fxs with
+               | pure xs => lengthM xs
+               | impure (ext (inl (sget _)) pf) =>
+                 pf (pget 42) >>= fun xs => lengthM xs
+               | impure (ext (inl (sput s'))   pf) =>
+                 pf (pput s') >>= fun xs => lengthM xs
+               | impure (ext (inr (inr sfail)) _)  => pure 0
+               | impure (ext (inr (inr (schoice mid))) pf) =>
+                 (pf true >>= fun xs => lengthM xs) >>= fun x =>
+                                                          (pf false >>= fun xs => lengthM xs) >>= fun y => pure (max x y)
+               | impure (ext (inr (inl (ssharing n)))  pf) =>
+                 pf (psharing n) >>= fun xs => lengthM xs
+               end
+      in m >>= fun i => pure (i + 1)
+    end.
+
+  Fixpoint convert (xs : list nat) : Prog (List nat) :=
+    match xs with
+    | nil => nilM
+    | cons x xs => consM (pure x) (convert xs)
+    end.
+End List.
