Coq/src/Classes.v
@@ -1,0 +1,11 @@
+Require Import Thesis.Prog.
+
+Class Shareable (A : Type) :=
+  {
+    shareArgs : A -> Prog A
+  }.
+
+Class Normalform (A B : Type) :=
+  {
+    nf : Prog A -> Prog B
+  }.
