Coq/src/Prog.v
@@ -1,0 +1,13 @@
+Require Import Thesis.Free.
+Require Import Thesis.Container.
+
+Export Thesis.Free.
+Export Thesis.Container.
+
+Definition NDShare := C__Comb (C__State nat) (C__Comb C__Sharing C__Choice).
+
+Definition NDShare__SC := C__Comb C__Sharing C__Choice.
+
+Definition Prog := Free NDShare.
+
+Definition Prog__SC := Free NDShare__SC.
